concurrency/fineConc_safe.v
@@ -22,6 +22,7 @@ Require Import compcert.lib.Integers.
 
 Require Import Coq.ZArith.ZArith.
 
+Require Import VST.concurrency.threadPool.
 Require Import VST.concurrency.dry_machine_lemmas.
 Require Import VST.concurrency.dry_machine_step_lemmas.
 Require Import VST.concurrency.threads_lemmas.
@@ -30,6 +31,7 @@ Require Import VST.concurrency.HybridMachineSig.
 Require Import VST.concurrency.mem_obs_eq.
 Require Import VST.concurrency.compcert_threads_lemmas.
 Require Import VST.concurrency.dry_context.
+Require Import VST.concurrency.tactics.
 Require Import Coqlib.
 Require Import VST.msl.Coqlib2.
 
@@ -43,10 +45,10 @@ Module FineConcInitial.
 
   Section FineConcInitial.
 
-  Context {Sem : Semantics}.
+    Context {Sem : Semantics}
+            {CI: CoreInj}.
 
   Variable init_mem : option Memory.Mem.mem.
-  Variable the_ge : semG.
 
   (** The initial memory is well-defined*)
   Parameter init_mem_wd:
@@ -54,12 +56,10 @@ Module FineConcInitial.
 
   (** The initial core is well-defined*)
   Parameter init_core_wd:
-    forall v args m (ARGS:valid_val_list (id_ren m) args),
+    forall c v args m (ARGS:valid_val_list (id_ren m) args),
       init_mem = Some m ->
-      match initial_core semSem 0 the_ge m v args with
-      | Some (c, _) => core_wd (id_ren m) c
-      | None => True
-      end.
+      initial_core semSem 0 m c v args ->
+      core_wd (id_ren m) c.
 
   (** The initial global env is well-defined*)
   Parameter the_ge_wd:
@@ -74,40 +74,55 @@ End FineConcInitial.
 (** ** Safety for FineConc (interleaving) semantics *)
 Module FineConcSafe.
 
-  Import AsmContext HybridMachineSig ThreadPoolWF.
-  Import Renamings MemObsEq ValObsEq ValueWD CoreInjections FineConcInitial ThreadPool.
-  Import Concur.mySchedule.
-  Import StepType.InternalSteps StepLemmas.
+  Import ThreadPool AsmContext ThreadPoolWF HybridMachine DryHybridMachine HybridMachineSig.
+  Import Renamings MemObsEq ValObsEq ValueWD CoreInjections FineConcInitial.
+  Import StepType InternalSteps StepLemmas.
 
   Import MemoryWD ThreadPoolInjections event_semantics.
 
   Section FineConcSafe.
 
-  Context {Sem : Semantics}.
+    Context {Sem : Semantics}
+            {semAx: CoreLanguage.SemAxioms}
+            {CI : CoreInj}.
 
   Variable init_mem : option Memory.Mem.mem.
-  Variable the_ge : semG.
 
   (** Excluded middle is required, but can be easily lifted*)
-  Axiom em : ClassicalFacts.excluded_middle.
+  Variable em : ClassicalFacts.excluded_middle.
 
   (* Is this the right instance? *)
-  Existing Instance Concur.DryMachineShell.
+  Existing Instance DryHybridMachine.dryResources.
+  Existing Instance DryHybridMachine.DryHybridMachineSig.
+  Existing Instance OrdinalPool.OrdinalThreadPool.
+  Existing Instance dryFineMach.
+  Existing Instance FineDilMem.
+  Existing Instance dryCoarseMach.
+  Existing Instance HybridFineMachine.scheduler.
+  Existing Instance HybridCoarseMachine.scheduler.
+  Existing Instance FineDilMem.
+  Existing Instance HybridCoarseMachine.DilMem.
 
   Lemma init_tp_wd:
-    forall v args m tp m' (ARGS:valid_val_list (id_ren m) args),
+    forall v args m tp (ARGS:valid_val_list (id_ren m) args),
       init_mem = Some m ->
-      init_mach(resources:=LocksAndResources) (init_perm init_mem) the_ge m v args = Some (tp, m') ->
+      @init_mach DryHybridMachine.dryResources _ _ _ (init_perm init_mem) m tp v args ->
       tp_wd (id_ren m) tp.
   Proof.
     intros.
     intros i cnti.
     simpl in H0.
-    unfold Concur.init_mach in H0.
-    destruct (initial_core semSem 0 the_ge m v args) as [[]|] eqn:?, init_perm; try discriminate.
-    inversion H0; subst.
-    simpl.
-    specialize (init_core_wd(init_mem := Some m) the_ge v ARGS). rewrite Heqo; auto.
+    unfold DryHybridMachine.init_mach in H0.
+    destruct H0 as [c [Hinit_core Hinit_perm]].
+    unfold init_perm in Hinit_perm.
+    rewrite H in Hinit_perm; subst.
+    unfold ctl_wd.
+    assert (Hget: getThreadC cnti = Krun c)
+      by (unfold getThreadC, OrdinalPool.getThreadC;
+          reflexivity).
+    rewrite Hget.
+    eapply init_core_wd;
+      now eauto.
   Qed.
 
   (** Assuming safety of cooperative VST.concurrency*)
@@ -116,51 +131,52 @@ Module FineConcSafe.
     Variables (f : val) (arg : list val) (initU : seq.seq nat).
 
     Variable init_coarse_safe:
-      forall  U tpc mem m sched n,
+      forall  U tpc mem sched n,
         init_mem = Some mem ->
-        tpc_init initU init_mem the_ge mem f arg = Some ((U, [::], tpc), m) ->
-        HybridCoarseMachine.csafe the_ge (sched,[::],tpc) mem n.
+        tpc_init initU init_mem mem (U, [::], tpc) f arg ->
+        HybridCoarseMachine.csafe (sched,[::],tpc) mem n.
 
   (** If the initial state is defined then the initial memory was also defined*)
   Lemma tpc_init_mem_defined:
     forall U tpc m,
-      tpc_init initU init_mem the_ge m f arg = Some (U, tpc) ->
+      tpc_init initU init_mem m (U, [::], tpc) f arg ->
       exists m, init_mem = Some m.
   Proof.
     unfold tpc_init. simpl.
-    unfold init_machine; simpl.
     unfold HybridMachine.DryHybridMachine.init_mach. intros.
+    destruct H as [? [Hinit Hinit_perm]].
     destruct init_perm eqn:?.
     unfold init_perm in *.
     destruct init_mem; try discriminate.
     eexists; reflexivity.
-    destruct (initial_core semSem 0 the_ge m f arg) as [[]|]; try discriminate.
+    destruct Hinit_perm;
+      now exfalso.
   Qed.
 
   (** [init_mach] and [init_mem] are related by [mem_compatible]*)
   Lemma init_compatible:
-    forall tp m m',
+    forall tp m,
       init_mem = Some m ->
-      init_mach(resources:=LocksAndResources) (init_perm init_mem) the_ge m f arg = Some (tp, m') ->
+      @init_mach DryHybridMachine.dryResources _ _ _ (init_perm init_mem) m tp f arg ->
       mem_compatible tp m.
   Proof.
     intros.
     destruct init_perm as [pmap|] eqn:Hinit_perm;
-      [| rewrite init_mach_none in H0; discriminate].
+      [| eapply init_mach_none in H0; now exfalso].
     unfold init_perm in Hinit_perm.
     rewrite H in Hinit_perm.
     inversion Hinit_perm; subst.
     constructor.
     - intros j cntj.
-      pose proof (init_thread _ _ _ _ H0 cntj); subst.
+      pose proof (init_thread H0 cntj); subst.
       erewrite getThreadR_init by eauto.
       simpl.
       split; [intros ? ?; now apply getCur_Max |now apply empty_LT].
     - intros.
-      erewrite init_lockRes_empty in H1 by eauto.
+      erewrite init_lockRes_empty in H by eauto.
       discriminate.
     - intros.
-      erewrite init_lockRes_empty in H1 by eauto.
+      erewrite init_lockRes_empty in H by eauto.
       discriminate.
   Qed.
 
@@ -168,23 +184,22 @@ Module FineConcSafe.
   Lemma init_mem_obs_eq :
     forall m tp i (cnti : containsThread tp i)
       (Hcomp: mem_compatible tp m)
-      (HcompF: mem_compatible tp (diluteMem m)),
+      (HcompF: mem_compatible tp (@diluteMem FineDilMem m)),
       init_mem = Some m ->
-      init_mach init_perm the_ge f arg = Some tp ->
-      mem_obs_eq (id_ren m) (restrPermMap (Hcomp _ cnti).1)
+      @init_mach DryHybridMachine.dryResources _ _ _ (init_perm init_mem) m tp f arg ->
+      mem_obs_eq (id_ren m) (restrPermMap (compat_th _ _ Hcomp cnti).1)
                  (restrPermMap (HcompF _ cnti).1) /\
       mem_obs_eq (id_ren m) (restrPermMap (Hcomp _ cnti).2)
                  (restrPermMap (HcompF _ cnti).2).
   Proof.
     intros.
     pose proof (mem_obs_eq_id (init_mem_wd H)) as Hobs_eq_id.
-    unfold init_mach in H0.
-    destruct (initial_core SEM.Sem 0 the_ge f arg), init_perm eqn:Hinit_perm;
-      try discriminate.
-    inversion H0; subst.
+    unfold init_mach in H0. simpl in H0.
+    unfold DryHybridMachine.init_mach in H0.
+    destruct H0 as [c [Hinit Hinit_perm]].
     unfold init_perm in Hinit_perm.
     rewrite H in Hinit_perm.
-    inversion Hinit_perm. subst.
+    subst tp.
     destruct Hobs_eq_id.
     split.
     - constructor.
@@ -202,12 +217,12 @@ Module FineConcSafe.
         do 2 rewrite restrPermMap_Cur.
         reflexivity.
         intros.
-        apply id_ren_correct in Hrenaming. subst.
+        apply id_ren_correct in Hrenaming. subst b2.
         eapply memval_obs_eq_id.
         apply Mem.perm_valid_block in Hperm.
         simpl.
         pose proof (init_mem_wd H Hperm ofs ltac:(reflexivity)).
-        destruct (ZMap.get ofs (Mem.mem_contents m) # b2); simpl; auto.
+        destruct (ZMap.get ofs (Mem.mem_contents m) # b1); simpl; auto.
         rewrite <- wd_val_valid; eauto.
         apply id_ren_domain.
         apply id_ren_correct.
@@ -228,8 +243,8 @@ Module FineConcSafe.
         intros.
         unfold Mem.perm in Hperm.
         pose proof (restrPermMap_Cur (Hcomp i cnti).2 b1 ofs).
-        unfold permission_at in H1.
-        rewrite H1 in Hperm.
+        unfold permission_at in H0.
+        rewrite H0 in Hperm.
         simpl in Hperm.
         rewrite empty_map_spec in Hperm.
         simpl in Hperm.
@@ -240,78 +255,97 @@ Module FineConcSafe.
   Lemma strong_tsim_refl:
     forall tp m i (cnti: containsThread tp i)
       (Hcomp: mem_compatible tp m)
-      (HcompF: mem_compatible tp (diluteMem m))
+      (HcompF: mem_compatible tp (@diluteMem FineDilMem m))
       (ARGS:valid_val_list (id_ren m) arg),
       init_mem = Some m ->
-      init_mach init_perm the_ge f arg = Some tp ->
-      strong_tsim (id_ren m) cnti cnti Hcomp HcompF.
+      @init_mach DryHybridMachine.dryResources _ _ _ (init_perm init_mem) m tp f arg ->
+      SimDefs.strong_tsim (id_ren m) cnti cnti Hcomp HcompF.
   Proof.
     intros.
     destruct (init_mem_obs_eq cnti Hcomp HcompF H H0).
     constructor; eauto.
     eapply ctl_inj_id; eauto.
-    apply (init_tp_wd _ ARGS H H0).
-    apply id_ren_correct.
+    apply (init_tp_wd ARGS H H0).
+    now apply id_ren_correct.
   Qed.
 
   Lemma setMaxPerm_inv:
-    forall m, max_inv (diluteMem m).
+    forall m, SimDefs.max_inv (@diluteMem FineDilMem m).
   Proof.
     intros.
-    unfold diluteMem, max_inv, Mem.valid_block, permission_at.
+    unfold diluteMem, SimDefs.max_inv, Mem.valid_block, permission_at.
+    simpl.
     intros b ofs H.
     simpl in H.
     apply setMaxPerm_MaxV with (ofs := ofs) in H.
     unfold permission_at in H.
-    auto.
+    now auto.
   Qed.
+
+  Lemma init_core_det:
+    forall h m f arg c c',
+      initial_core semSem h m c f arg ->
+      initial_core semSem h m c' f arg ->
+      c = c'.
+  Proof.
+  Admitted.
 
   (** Establishing the simulation relation for the initial state*)
   Lemma init_sim:
     forall U U' tpc tpf m n (ARG:valid_val_list (id_ren m) arg),
-      tpc_init f arg = Some (U, [::], tpc) ->
-      tpf_init f arg = Some (U', [::], tpf) ->
+      tpc_init initU init_mem m (U, [::], tpc) f arg ->
+      tpc_init initU init_mem m (U', [::], tpf) f arg ->
       init_mem = Some m ->
-      sim tpc m tpf (diluteMem m) nil (id_ren m) (id_ren m) (fun i cnti => id_ren m) n.
+      SimDefs.sim tpc [::] m tpf [::] (@diluteMem FineDilMem m) nil (id_ren m) (id_ren m) (fun i cnti => id_ren m) n.
   Proof.
-    intros.
+    intros.    
     unfold tpc_init, tpf_init in *. simpl in *.
-    unfold DryConc.init_machine, FineConc.init_machine in *.
-    destruct (init_mach init_perm the_ge f arg) eqn:Hinit; try discriminate.
-    inversion H; subst. inversion H0; subst.
-    clear H H0.
-    assert (HmemComp := init_compatible H1 Hinit).
-    assert (HmemCompF: mem_compatible tpf (diluteMem m))
+    destruct H as [? HinitC].
+    destruct H0 as [? HinitF].
+    assert (HmemComp := init_compatible H1 HinitC).
+    assert (HmemCompF0 := init_compatible H1 HinitF).
+    pose proof HinitC as HinitC'.
+    unfold DryHybridMachine.init_mach in HinitC, HinitF.
+    destruct HinitC as [cc [HinitC Hinit_permC]].
+    destruct HinitF as [cf [HinitF Hinit_permF]].
+    unfold init_perm in *.
+    rewrite H1 in Hinit_permF Hinit_permC.
+    assert (HmemCompF: mem_compatible tpf (@diluteMem FineDilMem m))
       by (eapply mem_compatible_setMaxPerm; eauto).
-    eapply Build_sim with (mem_compc := HmemComp) (mem_compf := HmemCompF).
+    subst tpf tpc U U'.
+    assert (cc = cf)
+      by (eapply init_core_det; now eauto).
+    subst cf.
+    eapply SimDefs.Build_sim with (mem_compc := HmemComp) (mem_compf := HmemCompF).
     - intros; split; auto.
     - simpl. rewrite addn0.
       intros.
       eapply init_coarse_safe with (n := n); eauto.
     - intros i cnti cnti'.
-      pose proof (strong_tsim_refl cnti HmemComp HmemCompF ARG H1 Hinit).
-      pf_cleanup.
-      destruct H. destruct obs_eq_data0, obs_eq_locks0.
-      constructor; eauto.
+      pose proof (strong_tsim_refl cnti HmemComp HmemCompF ARG H1 HinitC').
+      Tactics.pf_cleanup.
+      destruct H. destruct obs_eq_data, obs_eq_locks.
+      constructor;
+        now eauto.
     - intros; by congruence.
     - intros.
-      exists tpf, m.
+      exists (@mkPool dryResources _ _  (Krun cc) ((getCurPerm m, empty_map)#1, empty_map)), m.
       split; eauto with renamings.
       split; eauto.
       split; first by constructor.
       split.
-      intros; pf_cleanup.
+      intros; Tactics.pf_cleanup.
       eapply strong_tsim_refl; eauto.
-      pose proof (init_thread _ _ _ _  Hinit pff); subst.
+      pose proof (init_thread HinitC' pff); subst tid.
       repeat (split; intros); try congruence.
-      + erewrite getThreadR_init
-          by (unfold init_perm in Hinit;
-              rewrite H1 in Hinit;
-              eauto).
+      + rewrite H1 in HinitC'.
+        erewrite getThreadR_init by eauto.
         simpl.
-        pose proof (strong_tsim_refl pfc HmemComp HmemCompF ARG H1 Hinit).
-        pf_cleanup.
-        destruct H0. destruct obs_eq_data0.
+        pose proof (strong_tsim_refl pfc HmemComp HmemCompF ARG  H1).
+        rewrite H1 in H0. simpl in H0.
+        specialize (H0 HinitC').
+        Tactics.pf_cleanup.
+        destruct H0. destruct obs_eq_data.
         destruct weak_obs_eq0.
         destruct (valid_block_dec m b2).
         * pose proof (domain_valid0 _ v) as Hmapped.
@@ -324,42 +358,44 @@ Module FineConcSafe.
           unfold permission_at.
           assumption.
       + erewrite getThreadR_init
-          by ( unfold init_perm in Hinit;
-               rewrite H1 in Hinit;
+          by ( unfold init_perm in HinitC';
+               rewrite H1 in HinitC';
                eauto).
         simpl.
         now apply empty_map_spec.
-    - unfold init_mach in *.
-      unfold init_perm in Hinit.
-      rewrite H1 in Hinit.
-      destruct (initial_core SEM.Sem 0 the_ge f arg); try discriminate.
-      inversion Hinit; subst.
+    - unfold DryHybridMachine.init_mach in *.
+      rewrite H1 in HinitC'.
+      destruct HinitC' as [c' [HinitC' Heq]].
       split.
       + intros.
         exfalso.
         unfold initial_machine, lockRes in *. simpl in *.
-        erewrite threadPool.find_empty in Hl1, Hl2.
+        unfold OrdinalPool.mkPool, OrdinalPool.lockRes in *.
+        simpl in Hl1, Hl2.
+        erewrite OrdinalPool.find_empty in Hl1, Hl2.
         discriminate.
       + split.
         * intros.
           unfold lockRes, initial_machine in H.
-          rewrite threadPool.find_empty in H.
+          unfold OrdinalPool.mkPool, OrdinalPool.lockRes in *.
+          simpl in H.
           now exfalso.
         * intros.
           apply id_ren_correct in H; subst.
           split; auto.
     - intros.
-      unfold init_mach, init_perm in Hinit.
-      rewrite H1 in Hinit.
-      destruct (initial_core SEM.Sem 0 the_ge f arg); try discriminate.
-      inversion Hinit; subst.
-      unfold lockRes, initial_machine in *. simpl.
-      rewrite threadPool.find_empty in H.
+      unfold DryHybridMachine.init_mach in HinitC'.
+      rewrite H1 in HinitC'.
+      destruct HinitC' as [c' [HinitC' Heq]].
+      unfold initial_machine, lockRes in *. simpl in *.
+      unfold OrdinalPool.mkPool, OrdinalPool.lockRes in *.
+      simpl in H.
+      erewrite OrdinalPool.find_empty in H.
       discriminate.
     - eapply ThreadPoolWF.initial_invariant;
         now eauto.
     - apply setMaxPerm_inv; auto.
-    - apply init_mem_wd; auto.
+    - apply (@init_mem_wd _ _ H1); eauto.
     - eapply init_tp_wd; eauto.
     - eapply the_ge_wd; eauto.
     - split; eauto with renamings.
@@ -369,44 +405,70 @@ Module FineConcSafe.
 
   (** Proof of safety of the FineConc machine*)
 
-  Notation fsafe := (FineConc.fsafe the_ge).
+  Notation fsafe := (@HybridFineMachine.fsafe _ _ _ _ FineDilMem).
 
   (** If a thread has reached an external then it cannot be in the
   list that denotes the delta of execution between the two machines *)
   Lemma at_external_not_in_xs:
-    forall tpc mc tpf mf xs f fg fp i n
-      (Hsim: sim tpc mc tpf mf xs f fg fp n)
-      (pffi: containsThread tpf i)
-      (Hexternal: pffi @ E),
-      ~ List.In i xs.
+    forall tpc trc mc tpf trf mf xs f fg fp i n
+      (Hsim: SimDefs.sim tpc trc mc tpf trf mf xs f fg fp n)
+      (pffi: containsThread tpf i),
+      let mrestr := restrPermMap (compat_th _ _ (SimDefs.mem_compf Hsim) pffi).1 in
+      forall (Hexternal: getStepType pffi mrestr Concurrent),
+        ~ List.In i xs.
   Proof.
     intros; intro Hin.
     destruct Hsim.
     assert (pfci: containsThread tpc i)
-      by (eapply numThreads0; eauto).
-    specialize (simStrong0 _ pfci pffi).
-    destruct simStrong0 as (tpc' & mc' & Hincr & _ & Hexec & Htsim & _).
+      by (eapply numThreads; eauto).
+    pose proof (simStrong _ pfci pffi) as HsimStrongi.
+    destruct HsimStrongi as (tpc' & mc' & Hincr & _ & Hexec & Htsim & _).
     assert (pfci' : containsThread tpc' i)
       by (eapply InternalSteps.containsThread_internal_execution; eauto).
-
     assert (HmemCompC': mem_compatible tpc' mc')
-      by (eapply InternalSteps.internal_execution_compatible with (tp := tpc); eauto).
+      by (eapply InternalSteps.internal_execution_compatible with (tp := tpc) (m := mc);
+          eauto; eapply Hexec).
     specialize (Htsim pfci' HmemCompC').
     destruct Htsim.
-    clear - Hexec code_eq0 Hexternal Hin.
+    clear - Hexec code_eq Hexternal Hin HmemCompC' obs_eq_data Hincr semAx.
     unfold getStepType in Hexternal.
-    eapply internal_execution_result_type with (cnti' := pfci') in Hexec; eauto.
+    pose proof Hexec as Hexec'.
+    eapply internal_execution_result_type with (cnti' := pfci') (Hcomp' := HmemCompC') in Hexec;
+      eauto.
     unfold getStepType in Hexec.
-    apply ctlType_inj in code_eq0.
-    rewrite Hexternal in code_eq0.
-    auto.
+    destruct fg_spec.
+    erewrite SimProofs.ctlType_inj with (f:= fp i pfci) in Hexec; eauto.
+    eapply ren_incr_trans; eauto.
+    - erewrite <- restrPermMap_mem_valid.
+      eapply SimProofs.internal_execution_wd; eauto.
+      destruct (simWeak _ pfci pffi).
+      erewrite restrPermMap_domain with (Hlt := (compat_th _ _ mem_compc pfci).1).
+      eapply weak_obs_eq_domain_ren; now eauto.
+      eapply ren_incr_domain_incr; now eauto.
   Qed.
 
+  Lemma getStepType_cases:
+    forall tp m i (cnti: containsThread tp i),
+      getStepType cnti m Concurrent \/
+      getStepType cnti m Internal \/
+      getStepType cnti m Halted \/
+      getStepType cnti m Suspend.
+  Proof.
+    intros.
+    unfold getStepType, ctlType.
+    destruct (getThreadC cnti); try auto.
+    destruct (at_external semSem s m) eqn:?; try auto.
+    destruct (em (exists i0, halted semSem s i0)) as [Hhalted | Hnothalted].
+    right; right; left; now eauto.
+    right; left; right; now eauto.
+  Qed.
+    
+      
   (** Simulation between the two machines implies safety*)
   Lemma fine_safe:
-    forall tpf tpc mf mc (g fg : memren) fp (xs : Sch) sched
-      (Hsim: sim tpc mc tpf mf xs g fg fp (S (size sched))),
-      fsafe tpf mf sched (S (size sched)).
+    forall tpf trf tpc trc mf mc (g fg : memren) fp xs sched
+      (Hsim: SimDefs.sim tpc trc mc tpf trf mf xs g fg fp (S (size sched))),
+      @fsafe tpf mf sched (S (size sched)).
   Proof.
     intros.
     generalize dependent xs.
@@ -414,57 +476,73 @@ Module FineConcSafe.
     generalize dependent tpf.
     generalize dependent fp.
     generalize dependent tpc.
+    generalize dependent trc.
+    generalize dependent trf.
     generalize dependent mc.
     generalize dependent g.
     induction sched as [|i sched]; intros; simpl; auto.
     econstructor; simpl; eauto.
-    destruct (containsThread_dec i tpf) as [cnti | invalid].
+    destruct (OrdinalPool.containsThread_dec i tpf) as [cnti | invalid].
     - (** By case analysis on the step type *)
-      destruct (getStepType cnti) eqn:Htype.
-      + pose proof (sim_internal [::] cnti Htype Hsim) as
-            (tpf' & m' & fp' & tr' & Hstep & Hsim').
-        specialize (Hstep sched).
-        specialize (IHsched _ _ _ _ _ _ _ Hsim').
-        econstructor 3; simpl; eauto.
+      pose proof (getStepType_cases (restrPermMap (compat_th _ _ (SimDefs.mem_compf Hsim) cnti).1)
+                                  cnti) as Htype.
+      destruct Htype as [Htype | [Htype | [Htype | Htype]]].
       + assert (~ List.In i xs)
           by (eapply at_external_not_in_xs; eauto).
-        pose proof (sim_external [::] cnti Htype H Hsim) as Hsim'.
-        destruct Hsim' as (? & ? & ? & ? & ? & ? & tr' & Hstep & Hsim'').
-        specialize (IHsched _ _ _ _ _ _ _ Hsim'').
+        pose proof (@SimProofs.sim_external _ _ _ initU init_mem  em _ _ _ _ _ _ _ _ _ _ _ _ cnti H Hsim Htype) as Hsim'.
+        destruct Hsim' as (tpc' & trc' & mc' & tpf' & mf' & f' & fp' & tr' & Hstep & Hsim'').
+        specialize (IHsched _ _ _ _ _ _ _ _ _ Hsim'').
         specialize (Hstep sched).
+        unfold corestep in Hstep.
+        simpl in Hstep.
+        eapply @HybridFineMachine.StepSafe with (dilMem := FineDilMem);
+          eauto.
+      + pose proof (@SimProofs.sim_internal _ _ _ initU init_mem _ _ _ _ _ _ _ _ _ _ _ _ cnti Hsim Htype) as
+            (tpf' & m' & fp' & tr' & Hstep & Hsim').
+        specialize (Hstep sched).
+        specialize (IHsched _ _ _ _ _ _ _ _ _ Hsim').
+        unfold corestep in Hstep.
+        simpl in Hstep.
         econstructor 3; simpl; eauto.
-      + pose proof (sim_halted [::] cnti Htype Hsim) as Hsim'.
+      + pose proof (@SimProofs.sim_halted _ _ initU init_mem _ _ _ _ _  _ _ _  _ _  _  _ cnti Hsim Htype) as Hsim'.
         destruct Hsim' as (tr' & Hstep & Hsim'').
-        specialize (IHsched _ _ _ _ _ _ _ Hsim'').
+        specialize (IHsched _ _ _ _ _ _ _ _ _ Hsim'').
         specialize (Hstep sched).
+        unfold corestep in Hstep.
+        simpl in Hstep.
         econstructor 3;
           eauto.
-      + pose proof (sim_suspend [::] cnti Htype Hsim) as
-            (? & ? & tpf' & m' & ? & ? & tr' & Hstep & Hsim').
-        specialize (IHsched _ _ _ _ _ _ _ Hsim').
+      + pose proof (@SimProofs.sim_suspend _ _ _ initU init_mem em _ _ _ _ _ _ _  _ _ _ _ _ cnti Hsim Htype) as
+            (tpc' & trc' & mc' & tpf' & mf' & f' & fp' & tr' & Hstep & Hsim').
+        specialize (IHsched _ _ _ _ _ _ _ _ _ Hsim').
         specialize (Hstep sched).
-        econstructor 3; simpl; eauto.
-    -  pose proof (sim_fail [::] invalid Hsim) as
+        unfold corestep in Hstep.
+        simpl in Hstep.
+        econstructor 3; simpl;
+          now eauto.
+    -  pose proof (@SimProofs.sim_fail _ _  initU init_mem _ _ _ _  _  _ _  _ _ _ _ _ invalid Hsim) as
           (tr' & Hstep & Hsim').
-       specialize (IHsched _ _ _ _ _ _ _ Hsim').
+       specialize (IHsched _ _ _ _ _ _ _ _ _ Hsim').
        specialize (Hstep sched).
+       unfold corestep in Hstep.
+       simpl in Hstep.
        econstructor 3; eauto.
        Unshelve. eapply [::].
   Qed.
 
   (** *** Safety preservation for the FineConc machine starting from the initial state*)
   Theorem init_fine_safe:
-    forall U tpf m
+    forall tpf m
       (Hmem: init_mem = Some m)
-      (Hinit: tpf_init f arg = Some (U, [::], tpf))
+      (Hinit: tpf_init initU init_mem m (initU, [::], tpf) f arg)
       (ARG: valid_val_list (id_ren m) arg),
-    forall (sched : Sch),
-      fsafe tpf (diluteMem m) sched (size sched).+1.
+    forall sched ,
+      fsafe tpf (@diluteMem FineDilMem m) sched (size sched).+1.
   Proof.
     intros.
     assert (Hsim := init_sim (size sched).+1 ARG Hinit Hinit Hmem).
-    clear - Hsim.
-    eapply fine_safe; now eauto.
+    eapply fine_safe;
+      now eauto.
   Qed.
 
   End Safety.
